\subsection{controllable canonical form (frequency $\rightarrow$ time)}
\titel{$A$ is diagonal:}
\begin{align*}
    G(s) = \frac{p_1}{s-\lambda_1} + \frac{p_2}{s-\lambda_2} + ... + \frac{p_n}{s-\lambda_n} + d\\
    A = \left[\begin{array}{c c c}
        \lambda_1 & & \\
         & \ddots & \\
         & & \lambda_n
    \end{array}\right]
    ,
    B = \left[\begin{array}{c}
        \sqrt{p_1}\\
        \vdots\\
        \sqrt{p_n}
    \end{array}\right]
    \\
    C = \left[\begin{array}{c c c}
        \sqrt{p_1} & \cdots & \sqrt{p_n}
    \end{array}\right]
    ,
    D = d
\end{align*}

\titel{general case:}
\begin{align*}
    G(s) &= \frac{b_{n-1}s^{n-1} + b_{n-2}s^{n-2} + \dots + b_0}{s^n + a_{n-1}s^{n-1} + \dots + a_0} + d\\
    A &= \left[\begin{array}{c c c c c}
        0 & 1 & 0 & \cdots & 0\\
        0 & 0 & 1 & \cdots & 0\\
        \vdots & \vdots & & \ddots & 1\\
        -a_0 & -a_1 & \cdots & & -a_{n-1}
    \end{array}\right]
    ,
    B = \left[\begin{array}{c}
        0\\
        0\\
        \vdots\\
        1
    \end{array}\right]
    \\
    C &= \left[\begin{array}{c c c c}
        b_0 & b_1 & \cdots & b_{n-1}
    \end{array}\right]
    ,
    D = d
\end{align*}